lib/steel/pulse/Pulse.Checker.WithInv.fst
@@ -1,0 +1,138 @@
+module Pulse.Checker.WithInv
+
+open Pulse.Syntax
+open Pulse.Typing
+open Pulse.Checker.Pure
+open Pulse.Checker.Base
+open Pulse.Checker.Prover
+open Pulse.Checker.Comp
+open Pulse.Show
+
+module T = FStar.Tactics.V2
+module P = Pulse.Syntax.Printer
+module RT = FStar.Reflection.Typing
+module MT = Pulse.Typing.Metatheory
+
+let rt_recheck (gg:env) (#g:T.env) (#e:T.term) (#ty: T.typ) () : T.Tac (RT.tot_typing g e ty) =
+  info gg (Some (T.range_of_term e))
+    (Printf.sprintf "Re-checking %s at type %s"
+      (T.term_to_string e)
+      (T.term_to_string ty));
+  match T.core_check_term g e ty T.E_Total with
+  | Some tok, _ -> RT.T_Token _ _ _ ()
+  | None, _ -> T.fail "Checker.WithInv: rt_recheck failed" // fixme add a range
+
+let recheck (#g:env) (#e:term) (#ty: typ) () : T.Tac (tot_typing g e ty) =
+  core_check_tot_term_with_expected_type g e ty
+
+let term_remove_inv (inv:vprop) (tm:term) : T.Tac term =
+  match tm.t with
+  | Tm_Star tm inv' ->
+    if eq_tm inv inv' then tm
+    else T.fail "term_remove_inv"
+
+  | _ ->
+    T.fail "term_remove_inv: not a star?"
+
+let st_comp_remove_inv (inv:vprop) (c:st_comp) : T.Tac st_comp =
+  { c with pre = term_remove_inv inv c.pre
+         ; post = term_remove_inv inv c.post }
+
+#push-options "--z3rlimit 25"
+
+let check
+  (g:env)
+  (pre:term)
+  (pre_typing:tot_typing g pre tm_vprop)
+  (post_hint:post_hint_opt g)
+  (res_ppname:ppname)
+  (t:st_term{Tm_WithInv? t.term})
+  (check:check_t)
+  : T.Tac (checker_result_t g pre post_hint) =
+  let Tm_WithInv {name=inv_tm; returns_inv; body} = t.term in
+
+  let post : post_hint_t =
+    match returns_inv, post_hint with
+    | None, Some p -> p
+    | Some p, None ->
+      Pulse.Checker.Base.intro_post_hint g None None p
+    | Some p, Some q ->
+      fail g (Some t.range) "Fatal: multiple posts hint on with_invariant"
+    | _, _ ->
+      fail g (Some t.range) "Fatal: no post hint on with_invariant"
+  in
+  let post_hint = Some post in
+
+  info g (Some t.range)
+    (Printf.sprintf "Checker.WithInv: using post hint = %s"
+        (show post_hint));
+
+  let (| inv_tm, eff, inv_tm_ty, inv_tm_typing |) = check_term g inv_tm in
+
+  if eff <> T.E_Total then
+    fail g (Some inv_tm.range) "Ghost effect on inv?";
+
+  (* Check the term without an expected type, and check that it's Tm_Inv p *)
+  let inv_p =
+    match inv_tm_ty.t with
+    | Tm_Inv p -> p
+    | _ -> fail g (Some inv_tm.range)
+                (Printf.sprintf "Does not have invariant type (%s)" (P.term_to_string inv_tm_ty))
+  in
+
+  (* Can this come from some inversion instead? *)
+  let inv_p_typing : tot_typing g inv_p tm_vprop = recheck () in
+
+  (* pre'/post' are extended with inv_p *)
+  let pre' : vprop = tm_star pre inv_p in
+  let pre'_typing : tot_typing g pre' tm_vprop = recheck () in
+  let post_p' : vprop = tm_star post.post inv_p in
+  let elab_ret_ty = elab_term post.ret_ty in
+  let post_p'_typing
+    : RT.tot_typing (elab_env g)
+                    (RT.(mk_abs elab_ret_ty T.Q_Explicit (elab_term post_p')))
+                    (RT.mk_arrow elab_ret_ty T.Q_Explicit (elab_term tm_vprop))
+    = rt_recheck g ()
+  in
+
+  (* the post hint for the body, extended with inv_p *)
+  let post' : post_hint_for_env g = { post with
+    g = g;
+    ty_typing = recheck (); // Pulse.Typing.Metatheory.tot_typing_weakening _ _ _ _ post.ty_typing _;
+    post = post_p';
+    post_typing = post_p'_typing;
+  }
+  in
+
+  let (| body, c_body, body_typing |) =
+    let ppname = mk_ppname_no_range "with_inv_body" in
+    let r = check g pre' pre'_typing (Some post') ppname body in
+    apply_checker_result_k r ppname
+  in
+  
+  info g (Some body.range)
+    (Printf.sprintf "Checked body at comp type %s"
+        (P.comp_to_string c_body));
+
+  let c_out : comp_st =
+    match c_body with
+    | C_ST st -> C_ST (st_comp_remove_inv inv_p st)
+    | C_STAtomic inames st -> C_STAtomic inames (st_comp_remove_inv inv_p st)
+    | C_STGhost inames st -> C_STGhost inames (st_comp_remove_inv inv_p st)
+  in
+  assume (add_inv c_out inv_p == c_body);
+
+  let tm : st_term =
+    { term = Tm_WithInv {name=inv_tm; body; returns_inv = None}; range = t.range }
+  in
+
+  let d : st_typing g tm c_out =
+    T_WithInv g inv_tm inv_p inv_p_typing inv_tm_typing body c_out body_typing
+  in
+  info g (Some body.range)
+
+    (Printf.sprintf "Returning comp type %s"
+        (P.comp_to_string c_out));
+
+
+  checker_result_for_st_typing (| tm, c_out, d |)  res_ppname
